src/proof/index.v
@@ -3,7 +3,7 @@ From New.proof Require Export apimodel list util.
 From New.proof.kubernetes_model Require Export apimodel_init.
 
 Section proof.
-Context `{!mapG Σ KKey.t PureKObject.t}.
+Context `{!mapG Σ KKey.t KObjectV.t}.
 Context `{!mapG Σ KKey.t (gset KKey.t)}.
 Context `{!auth_setG Σ KKey.t}.
 Context `{hG: !heapGS Σ} {go_ctx: GoContext}.
@@ -13,21 +13,21 @@ Lemma wp_index_of_podController index_name obj ptr pod pure_pod dq:
       "%Hindex_name" ∷ ⌜ index_name = "podController"%go ⌝ ∗
       "%Hobj" ∷ ⌜ obj = interface.mk (ptrT.id v1.Pod.id) #ptr ⌝ ∗
       "Hptr" ∷ ptr ↦{dq} pod ∗
-      "Hdeepown_pod" ∷ PurePod.deepown pod pure_pod dq ∗
-      "%Hwf" ∷ ⌜ PurePod.well_formed pure_pod ⌝
+      "Hdeepown_pod" ∷ PodV.deepown pod pure_pod dq ∗
+      "%Hwf" ∷ ⌜ PodV.well_formed pure_pod ⌝
   }}}
     @! apimodel.index_of #index_name #obj
   {{{ sl idx_val_list idx_val, RET (#sl, #interface.nil);
       sl ↦* idx_val_list ∗
       ⌜ idx_val_list = [idx_val] ⌝ ∗
       ⌜ ∀ parent_kind parent_name parent_uid,
-        obj_has_controller_parent_of (PureKObject.Pod pure_pod) parent_kind parent_name parent_uid ↔
-        idx_val = pure_pod.(PurePod.ObjectMeta').(PureObjectMeta.Namespace') ++ "/"%go ++
+        obj_has_controller_parent_of (KObjectV.Pod pure_pod) parent_kind parent_name parent_uid ↔
+        idx_val = pure_pod.(PodV.ObjectMeta').(ObjectMetaV.Namespace') ++ "/"%go ++
                   parent_kind ++ "/"%go ++ parent_name ++ "/"%go ++ parent_uid ⌝ ∗
-      ⌜ idx_val = pure_pod.(PurePod.ObjectMeta').(PureObjectMeta.Namespace') ∨ (* the orphan case *)
-        ∃ suffix, idx_val = pure_pod.(PurePod.ObjectMeta').(PureObjectMeta.Namespace') ++ "/"%go ++ suffix ⌝ ∗
+      ⌜ idx_val = pure_pod.(PodV.ObjectMeta').(ObjectMetaV.Namespace') ∨ (* the orphan case *)
+        ∃ suffix, idx_val = pure_pod.(PodV.ObjectMeta').(ObjectMetaV.Namespace') ++ "/"%go ++ suffix ⌝ ∗
       ptr ↦{dq} pod ∗
-      PurePod.deepown pod pure_pod dq
+      PodV.deepown pod pure_pod dq
   }}}.
 Proof. Admitted.
 
@@ -39,24 +39,24 @@ Lemma wp_State__ByIndex_pod γ l kind index_name indexed_value parent_key parent
       "%Hindexed_value" ∷ ⌜ indexed_value = parent_key.(KKey.Namespace') ++ "/"%go ++
                                             parent_key.(KKey.Kind') ++ "/"%go ++
                                             parent_key.(KKey.Name') ++ "/"%go ++
-                                            (PureKObject.objectmeta parent).(PureObjectMeta.UID') ⌝ ∗
+                                            (KObjectV.objectmeta parent).(ObjectMetaV.UID') ⌝ ∗
       "Hghost_parent" ∷ parent_key [[ γ.(γ_state) ]]↦ parent ∗
-      "Hghost_pure_pod_map" ∷ ([∗ map] key ↦ pod ∈ pure_pod_map, key [[ γ.(γ_state) ]]↦ PureKObject.Pod pod) ∗
+      "Hghost_pure_pod_map" ∷ ([∗ map] key ↦ pod ∈ pure_pod_map, key [[ γ.(γ_state) ]]↦ KObjectV.Pod pod) ∗
       "Hghost_children_keys" ∷ parent_key [[ γ.(γ_children) ]]↦ children_keys ∗
       "%Hdom_eq" ∷ ⌜ children_keys = dom pure_pod_map ⌝
   }}}
     l @ (ptrT.id apimodel.State.id) @ "ByIndex" #kind #index_name #indexed_value
-  {{{ objs_l (ptr_list: list loc) (pure_pod_list: list PurePod.t) dq, RET (#objs_l, #interface.nil);
+  {{{ objs_l (ptr_list: list loc) (pure_pod_list: list PodV.t) dq, RET (#objs_l, #interface.nil);
       "Hobjs_l" ∷ objs_l ↦* map (λ ptr, interface.mk (ptrT.id v1.Pod.id) #ptr) ptr_list ∗
-      "Hptrs_purepods" ∷ ([∗ list] ptr;pure_pod ∈ ptr_list;pure_pod_list, ∃ pod, ptr ↦{dq} pod ∗ PurePod.deepown pod pure_pod dq) ∗
-      "%Hwf_pure_pod_list" ∷ ⌜ ∀ p, p ∈ pure_pod_list → PurePod.well_formed p ⌝ ∗
-      "%Hlist_in_map" ∷  ⌜ ∀ p, p ∈ pure_pod_list → pure_pod_map !! (PurePod.key p) = Some p ⌝ ∗
+      "Hptrs_purepods" ∷ ([∗ list] ptr;pure_pod ∈ ptr_list;pure_pod_list, ∃ pod, ptr ↦{dq} pod ∗ PodV.deepown pod pure_pod dq) ∗
+      "%Hwf_pure_pod_list" ∷ ⌜ ∀ p, p ∈ pure_pod_list → PodV.well_formed p ⌝ ∗
+      "%Hlist_in_map" ∷  ⌜ ∀ p, p ∈ pure_pod_list → pure_pod_map !! (PodV.key p) = Some p ⌝ ∗
       "%Hmap_in_list" ∷ ⌜ ∀ k p, pure_pod_map !! k = Some p → p ∈ pure_pod_list ⌝ ∗
-      "%Hown_pod_keys_eq" ∷ ⌜ ∀ key pod, pure_pod_map !! key = Some pod → key = PurePod.key pod ⌝ ∗
-      "%Hno_dup" ∷ ⌜ ∀ i j p1 p2, i ≠ j → pure_pod_list !! i = Some p1 → pure_pod_list !! j = Some p2 → (PurePod.key p1) ≠ (PurePod.key p2) ⌝ ∗
+      "%Hown_pod_keys_eq" ∷ ⌜ ∀ key pod, pure_pod_map !! key = Some pod → key = PodV.key pod ⌝ ∗
+      "%Hno_dup" ∷ ⌜ ∀ i j p1 p2, i ≠ j → pure_pod_list !! i = Some p1 → pure_pod_list !! j = Some p2 → (PodV.key p1) ≠ (PodV.key p2) ⌝ ∗
       "%Hpure_pod_map_namespace_eq" ∷ ⌜ ∀ key, key ∈ dom pure_pod_map → key.(KKey.Namespace') = parent_key.(KKey.Namespace') ⌝ ∗
       "Hghost_parent" ∷ parent_key [[ γ.(γ_state) ]]↦ parent ∗
-      "Hghost_pure_pod_map" ∷ ([∗ map] key ↦ pod ∈ pure_pod_map, key [[ γ.(γ_state) ]]↦ PureKObject.Pod pod) ∗
+      "Hghost_pure_pod_map" ∷ ([∗ map] key ↦ pod ∈ pure_pod_map, key [[ γ.(γ_state) ]]↦ KObjectV.Pod pod) ∗
       "Hghost_children_keys" ∷ parent_key [[ γ.(γ_children) ]]↦ children_keys
   }}}.
 Proof.
@@ -72,7 +72,7 @@ Proof.
   { iPureIntro. split; [done|]. destruct Hinv_Hghost_well_formed. done. }
   iIntros (sl ptr_list pure_pod_list) "(Hsl & Hlist & %Hwf & %Hlookup_abs & %Hno_dup & %Hns_match & %Hmap_in_list &
     Hinv_Hstate_m_addr & Hinv_Hown_phys & Hinv_Hown_abs & Hinv_Hphys_abs_rep & Hghost_pure_pod_map)". wp_auto.
-  assert (∀ (k : KKey.t) (p : PurePod.t), pure_pod_map !! k = Some p → p ∈ pure_pod_list) as Hmap_in_list'.
+  assert (∀ (k : KKey.t) (p : PodV.t), pure_pod_map !! k = Some p → p ∈ pure_pod_list) as Hmap_in_list'.
   { intros k p Hlookup. apply (Hmap_in_list k p Hlookup). unfold namespace_matches. left. done. }
   clear Hns_match. rename Hmap_in_list' into Hns_match.
   set obj_list := map (λ ptr : loc, interface.mk (ptrT.id v1.Pod.id) (# ptr)) ptr_list.
@@ -83,14 +83,14 @@ Proof.
   iDestruct (own_slice_len with "Hsl") as %(Hsl_len1 & Hsl_len2).
   iDestruct (own_slice_wf with "Hsl") as %Hsl_cap.
   iDestruct (big_sepL2_length with "Hlist") as %Hlen_ptr_pure_pod.
-  set P := (λ p, obj_has_controller_parent_of (PureKObject.Pod p) parent_key.(KKey.Kind') parent_key.(KKey.Name') (PureKObject.objectmeta parent).(PureObjectMeta.UID')).
-  set I := (∃ (i: w64) (val: interface.t) (sl': slice.t) (ptr_list': list loc) (pure_pod_list': list PurePod.t),
+  set P := (λ p, obj_has_controller_parent_of (KObjectV.Pod p) parent_key.(KKey.Kind') parent_key.(KKey.Name') (KObjectV.objectmeta parent).(ObjectMetaV.UID')).
+  set I := (∃ (i: w64) (val: interface.t) (sl': slice.t) (ptr_list': list loc) (pure_pod_list': list PodV.t),
     "Hi_ptr" ∷ i_ptr ↦ i ∗
     "Hval_ptr" ∷ val_ptr ↦ val ∗
     "Hitems_ptr" ∷ items_ptr ↦ sl' ∗
     "Hsl'" ∷ sl' ↦* map (λ ptr : loc, interface.mk (ptrT.id v1.Pod.id) (# ptr)) ptr_list' ∗
-    "Hlist_pre" ∷ ([∗ list] ptr;pure_pod ∈ ptr_list';pure_pod_list', ∃ pod, PurePod.deepown_l ptr pod pure_pod 1) ∗
-    "Hlist_post" ∷ ([∗ list] ptr;pure_pod ∈ (drop (sint.nat i) ptr_list);(drop (sint.nat i) pure_pod_list), ∃ pod, PurePod.deepown_l ptr pod pure_pod 1) ∗
+    "Hlist_pre" ∷ ([∗ list] ptr;pure_pod ∈ ptr_list';pure_pod_list', ∃ pod, PodV.deepown_l ptr pod pure_pod 1) ∗
+    "Hlist_post" ∷ ([∗ list] ptr;pure_pod ∈ (drop (sint.nat i) ptr_list);(drop (sint.nat i) pure_pod_list), ∃ pod, PodV.deepown_l ptr pod pure_pod 1) ∗
     "Hcap_sl'" :: own_slice_cap interface.t sl' (DfracOwn 1) ∗
     "%Hfilter_ptr_list" ∷ ⌜ pure_pod_list' = filter P (take (sint.nat i) pure_pod_list) ⌝ ∗
     "%Hi" ∷ ⌜ 0 ≤ sint.Z i ≤ sint.Z (slice.len_f sl) ⌝
@@ -116,7 +116,7 @@ Proof.
         injection Hthis_obj_lookup. done.
       - apply Hwf. apply (list_elem_of_lookup_2 _ (sint.nat i)). done. }
     iIntros (sl0 idx_val_list idx_val) "(Hsl0 & -> & %Hidx_val & %Hidx_val_prefix & Hthis_ptr & Hdeepown_this_pod)". wp_auto.
-    specialize Hidx_val with parent_key.(KKey.Kind') parent_key.(KKey.Name') (PureKObject.objectmeta parent).(PureObjectMeta.UID').
+    specialize Hidx_val with parent_key.(KKey.Kind') parent_key.(KKey.Name') (KObjectV.objectmeta parent).(ObjectMetaV.UID').
     rewrite bool_decide_true //. wp_auto.
     wp_alloc j_ptr as "Hj_ptr". wp_auto.
     iDestruct (own_slice_len with "Hsl0") as %(Hsl0_len1 & _). simpl in Hsl0_len1.
@@ -137,23 +137,23 @@ Proof.
       wp_apply (wp_load_slice_elem with "[$Hsl0]"); [word| | ].
       { iPureIntro. assert (sint.nat j = 0%nat) as -> by word. done. }
       iIntros "Hsl0". wp_auto.
-      assert (P this_pure_pod ↔ idx_val = PureObjectMeta.Namespace' (PurePod.ObjectMeta' this_pure_pod) ++ "/"%go ++
+      assert (P this_pure_pod ↔ idx_val = ObjectMetaV.Namespace' (PodV.ObjectMeta' this_pure_pod) ++ "/"%go ++
                                           parent_key.(KKey.Kind') ++ "/"%go ++
                                           parent_key.(KKey.Name') ++ "/"%go ++
-                                          (PureKObject.objectmeta parent).(PureObjectMeta.UID')) as Hidx_val'.
+                                          (KObjectV.objectmeta parent).(ObjectMetaV.UID')) as Hidx_val'.
       { unfold P. apply Hidx_val. }
       simpl in Hidx_val'.
       destruct (bool_decide(P this_pure_pod)) eqn:HP.
       * apply bool_decide_eq_true in HP.
-        assert (this_pure_pod.(PurePod.ObjectMeta').(PureObjectMeta.Namespace') = parent_key.(KKey.Namespace')) as Hns_eq.
+        assert (this_pure_pod.(PodV.ObjectMeta').(ObjectMetaV.Namespace') = parent_key.(KKey.Namespace')) as Hns_eq.
         { destruct Hinv_Hghost_well_formed. 
-          assert (this_pure_pod.(PurePod.ObjectMeta').(PureObjectMeta.Namespace') = (PurePod.key this_pure_pod).(KKey.Namespace')) as -> by done.
+          assert (this_pure_pod.(PodV.ObjectMeta').(ObjectMetaV.Namespace') = (PodV.key this_pure_pod).(KKey.Namespace')) as -> by done.
           symmetry.
           apply (Hparents_children_same_namespace _ (dom pure_pod_map) _ Hlookup_children).
           pose proof (split_children_point_to_parent _ _ Hchildren_point_to_parent) as [Hchildren_point_to_parent1 Hchildren_point_to_parent2].
-          assert (abs_state !! PurePod.key this_pure_pod = Some (PureKObject.Pod this_pure_pod)) as Hlookup_abs'.
+          assert (abs_state !! PodV.key this_pure_pod = Some (KObjectV.Pod this_pure_pod)) as Hlookup_abs'.
           { apply Hlookup_abs. apply (list_elem_of_lookup_2 _ (sint.nat i)). done. }
-          apply (Hchildren_point_to_parent1 parent_key parent (PurePod.key this_pure_pod) (PureKObject.Pod this_pure_pod)).
+          apply (Hchildren_point_to_parent1 parent_key parent (PodV.key this_pure_pod) (KObjectV.Pod this_pure_pod)).
           all: try done. }
         rewrite bool_decide_true //.
         { rewrite <-Hns_eq. apply Hidx_val'. done. }
@@ -185,20 +185,20 @@ Proof.
         iFrame.
       * apply bool_decide_eq_false in HP.
         rewrite bool_decide_false //.
-        { destruct (bool_decide(this_pure_pod.(PurePod.ObjectMeta').(PureObjectMeta.Namespace') = parent_key.(KKey.Namespace'))) eqn:Hns.
+        { destruct (bool_decide(this_pure_pod.(PodV.ObjectMeta').(ObjectMetaV.Namespace') = parent_key.(KKey.Namespace'))) eqn:Hns.
           -- apply bool_decide_eq_true in Hns. rewrite <-Hns. intros Heq. apply HP. apply Hidx_val'. done.
-          -- assert (slash_free (PureObjectMeta.Namespace' (PurePod.ObjectMeta' this_pure_pod))) as Hslash_free1.
+          -- assert (slash_free (ObjectMetaV.Namespace' (PodV.ObjectMeta' this_pure_pod))) as Hslash_free1.
             { apply valid_namespace_slash_free.
-              assert (PurePod.well_formed this_pure_pod) as Hwf_pod.
+              assert (PodV.well_formed this_pure_pod) as Hwf_pod.
               { apply Hwf. apply (list_elem_of_lookup_2 _ (sint.nat i)). done. }
-              destruct Hwf_pod as [Hwf_meta _]. unfold PureObjectMeta.well_formed in Hwf_meta. intuition. }
+              destruct Hwf_pod as [Hwf_meta _]. unfold ObjectMetaV.well_formed in Hwf_meta. intuition. }
             assert (slash_free (KKey.Namespace' parent_key)) as Hslash_free2.
             { apply valid_namespace_slash_free.
               destruct Hinv_Hghost_well_formed. 
               pose proof Habs_state_well_formed parent_key parent Hlookup_abs_parent as [Hparent_key Hwf_parent].
               pose proof well_formed_object_has_well_formed_key parent_key parent Hparent_key Hwf_parent as Hwf_key.
               intuition. }
-            assert (PureObjectMeta.Namespace' (PurePod.ObjectMeta' this_pure_pod) ≠ KKey.Namespace' parent_key) as Hneq.
+            assert (ObjectMetaV.Namespace' (PodV.ObjectMeta' this_pure_pod) ≠ KKey.Namespace' parent_key) as Hneq.
             { intros H. apply bool_decide_eq_false in Hns. done. }
             destruct Hidx_val_prefix as [Hidx_val_prefix|Hidx_val_prefix].
             ++ rewrite Hidx_val_prefix. apply pod_controller_index_key_inequality1. all: done.
@@ -223,13 +223,13 @@ Proof.
         destruct (decide (P this_pure_pod)); [done|].
         rewrite filter_nil app_nil_r. done. }
       iFrame.
-  - iAssert (⌜ ∀ key pod, pure_pod_map !! key = Some pod → abs_state !! key = Some (PureKObject.Pod pod) ⌝%I)
+  - iAssert (⌜ ∀ key pod, pure_pod_map !! key = Some pod → abs_state !! key = Some (KObjectV.Pod pod) ⌝%I)
     as "%Hsub_map".
-    { iAssert (⌜ fmap PureKObject.Pod pure_pod_map ⊆ abs_state ⌝%I) as %Hsubset.
+    { iAssert (⌜ fmap KObjectV.Pod pure_pod_map ⊆ abs_state ⌝%I) as %Hsubset.
       { iApply (map_valid_subset with "Hinv_Hown_abs").
         rewrite big_sepM_fmap. iFrame "Hghost_pure_pod_map". }
       iPureIntro. intros key pod Hlookup.
-      assert ((fmap PureKObject.Pod pure_pod_map) !! key = Some (PureKObject.Pod pod)) as Hlookup_fmap.
+      assert ((fmap KObjectV.Pod pure_pod_map) !! key = Some (KObjectV.Pod pod)) as Hlookup_fmap.
       { rewrite lookup_fmap. rewrite Hlookup. done. }
       eapply lookup_weaken; [exact Hlookup_fmap|exact Hsubset]. }
     iCombineNamed "Hinv_*" as "H".
@@ -244,7 +244,7 @@ Proof.
       pose proof Hsub_map key pod Hlookup as Hlookup'.
       assert (key ∈ (dom pure_pod_map)) as Hkeyin.
       { apply elem_of_dom. exists pod. done. }
-      pose proof Hchildren_point_to_parent parent_key parent key (PureKObject.Pod pod) (dom pure_pod_map)
+      pose proof Hchildren_point_to_parent parent_key parent key (KObjectV.Pod pod) (dom pure_pod_map)
         Hlookup_abs_parent Hlookup' Hlookup_children as Hbi.
       pose proof (proj1 Hbi) Hkeyin as Hobj_has_controller_parent_of. done. }
     split_and!.
@@ -252,15 +252,15 @@ Proof.
     * intros p Hlookup_list. apply list_elem_of_filter in Hlookup_list as [HPp Hlookup_list].
       pose proof Hlookup_abs p Hlookup_list as Hlookup_abs'.
       destruct Hinv_Hghost_well_formed.
-      pose proof Hchildren_point_to_parent parent_key parent (PurePod.key p) (PureKObject.Pod p)
+      pose proof Hchildren_point_to_parent parent_key parent (PodV.key p) (KObjectV.Pod p)
         (dom pure_pod_map) Hlookup_abs_parent Hlookup_abs' Hlookup_children as Hbi.
       pose proof (proj2 Hbi) HPp as Hkey_in_dom. apply elem_of_dom in Hkey_in_dom as [p' Hlookup_map].
-      pose proof Hsub_map (PurePod.key p) p' Hlookup_map as Hlookup_abs''.
+      pose proof Hsub_map (PodV.key p) p' Hlookup_map as Hlookup_abs''.
       rewrite Hlookup_abs' in Hlookup_abs''. injection Hlookup_abs''. intros ->. done.
     * intros k p Hlookup. pose proof HmapP k p Hlookup as HPp. apply list_elem_of_filter. split; [done|].
       pose proof Hns_match k p Hlookup. done.
     * intros k p Hlookup. destruct Hinv_Hghost_well_formed. pose proof Hsub_map k p Hlookup as Hlookup'.
-      pose proof Habs_state_well_formed k (PureKObject.Pod p) Hlookup' as Hwf'. destruct Hwf' as [Hwf' _]. done.
+      pose proof Habs_state_well_formed k (KObjectV.Pod p) Hlookup' as Hwf'. destruct Hwf' as [Hwf' _]. done.
     * apply filter_preserves_key_uniqueness. done.
     * intros k Hkindom. destruct Hinv_Hghost_well_formed. symmetry.
       apply (Hparents_children_same_namespace _ (dom pure_pod_map)); [done|done].
