src/proof/new.v
@@ -10,29 +10,27 @@ From New.proof.big_op Require Export big_sepL big_sepM.
 Section spec.
 Context `{hG: !heapGS Σ} {go_ctx: GoContext}.
 
-Axiom own_meta_frag: gname → KKey.t → types.UID.t → option PureObjectMeta.t → iProp Σ.
+Axiom own_meta_frag: gname → KKey.t → types.UID.t → option ObjectMetaV.t → iProp Σ.
 
-Axiom own_weak_spec_frag: gname → KKey.t → types.UID.t → PureObjectSpec.t → iProp Σ.
+Axiom own_weak_spec_frag: gname → KKey.t → types.UID.t → ObjectSpecV.t → iProp Σ.
 
-Axiom own_weak_status_frag: gname → KKey.t → types.UID.t → PureObjectStatus.t → iProp Σ.
+Axiom own_weak_status_frag: gname → KKey.t → types.UID.t → ObjectStatusV.t → iProp Σ.
 
 Axiom own_weak_children_frag: gname → KKey.t → types.UID.t → gset KKey.t → iProp Σ.
 
 Axiom own_fresh_key_frag: gname → KKey.t → iProp Σ.
 
 (* A snapshot of the object given the key, uid, and rv. It's persistent. *)
-Axiom own_snapshot_ro_frag: gname → KKey.t → types.UID.t → go_string → PureKObject.t → iProp Σ.
+Axiom own_snapshot_ro_frag: gname → KKey.t → types.UID.t → go_string → KObjectV.t → iProp Σ.
 
 Definition own_snapshot_ro_frag_of γ kobj: iProp Σ :=
   own_snapshot_ro_frag γ
-    (PureKObject.key kobj)
-    (PureKObject.objectmeta kobj).(PureObjectMeta.UID')
-    (PureKObject.objectmeta kobj).(PureObjectMeta.ResourceVersion')
+    (KObjectV.key kobj)
+    (KObjectV.objectmeta kobj).(ObjectMetaV.UID')
+    (KObjectV.objectmeta kobj).(ObjectMetaV.ResourceVersion')
     kobj.
 
 Axiom is_kubernetes: gname → loc → iProp Σ. (* Kubernetes invariant *)
-
-Axiom valid: PureKObject.t → Prop.
 
 Lemma wp_State__get γ l key:
   {{{ is_pkg_init apimodel ∗
@@ -41,9 +39,9 @@ Lemma wp_State__get γ l key:
     l @ (ptrT.id apimodel.State.id) @ "get" #key
   {{{ i (err: error.t) kobj, RET (#i, #err);
       ( ⌜ err = interface.nil ⌝ ∗
-        ⌜ valid kobj ⌝ ∗
-        ⌜ key = PureKObject.key kobj ⌝ ∗
-        PureKObject.deepown_i i kobj 1 ∗
+        ⌜ KObjectV.valid kobj ⌝ ∗
+        ⌜ key = KObjectV.key kobj ⌝ ∗
+        KObjectV.deepown_i i kobj 1 ∗
         own_snapshot_ro_frag_of γ kobj
       ) ∨
       ⌜ err ≠ interface.nil ⌝
@@ -58,10 +56,10 @@ Lemma wp_State__get_none γ l key uid:
     l @ (ptrT.id apimodel.State.id) @ "get" #key
   {{{ i (err: error.t) kobj, RET (#i, #err);
       (( ⌜ err = interface.nil ⌝ ∗
-          ⌜ valid kobj ⌝ ∗
-          ⌜ key = PureKObject.key kobj ⌝ ∗
-          ⌜ uid ≠ (PureKObject.objectmeta kobj).(PureObjectMeta.UID') ⌝ ∗
-          PureKObject.deepown_i i kobj 1 ∗
+          ⌜ KObjectV.valid kobj ⌝ ∗
+          ⌜ key = KObjectV.key kobj ⌝ ∗
+          ⌜ uid ≠ (KObjectV.objectmeta kobj).(ObjectMetaV.UID') ⌝ ∗
+          KObjectV.deepown_i i kobj 1 ∗
           own_snapshot_ro_frag_of γ kobj
         ) ∨
         ⌜ err ≠ interface.nil ⌝
@@ -73,7 +71,7 @@ Proof. Admitted.
 Lemma wp_State__get_some γ l key uid kmeta kspec_o kstatus_o:
   {{{ is_pkg_init apimodel ∗
       "#Hisk" ∷ is_kubernetes γ l ∗
-      "%Huid" ∷ ⌜ uid = kmeta.(PureObjectMeta.UID') ⌝ ∗
+      "%Huid" ∷ ⌜ uid = kmeta.(ObjectMetaV.UID') ⌝ ∗
       "Hmeta" ∷ own_meta_frag γ key uid (Some kmeta) ∗
       "Hspec" ∷ (match kspec_o with
                   | Some kspec => own_weak_spec_frag γ key uid kspec
@@ -86,53 +84,49 @@ Lemma wp_State__get_some γ l key uid kmeta kspec_o kstatus_o:
   }}}
     l @ (ptrT.id apimodel.State.id) @ "get" #key
   {{{ i kobj, RET (#i, #interface.nil);
-      ⌜ valid kobj ⌝ ∗
-      ⌜ key = PureKObject.key kobj ⌝ ∗
-      ⌜ kmeta = PureKObject.objectmeta kobj ⌝ ∗
-      PureKObject.deepown_i i kobj 1 ∗
+      ⌜ KObjectV.valid kobj ⌝ ∗
+      ⌜ key = KObjectV.key kobj ⌝ ∗
+      ⌜ kmeta = KObjectV.objectmeta kobj ⌝ ∗
+      KObjectV.deepown_i i kobj 1 ∗
       own_meta_frag γ key uid (Some kmeta) ∗
       (match kspec_o with
-      | Some kspec => own_weak_spec_frag γ key uid kspec ∗ ⌜ kspec = PureKObject.spec kobj ⌝
+      | Some kspec => own_weak_spec_frag γ key uid kspec ∗ ⌜ kspec = KObjectV.spec kobj ⌝
       | None => True
       end) ∗
       (match kstatus_o with
-      | Some kstatus => own_weak_status_frag γ key uid kstatus ∗ ⌜ kstatus = PureKObject.status kobj ⌝
+      | Some kstatus => own_weak_status_frag γ key uid kstatus ∗ ⌜ kstatus = KObjectV.status kobj ⌝
       | None => True
       end) ∗
       own_snapshot_ro_frag_of γ kobj
   }}}.
 Proof. Admitted.
 
-Axiom valid_create: go_string → PureKObject.t → Prop.
-
-Axiom valid_nameless_create: go_string → PureKObject.t → Prop.
-
 Lemma wp_State__create γ l kind namespace i kobj key parent_key parent_uid parent_meta children:
   {{{ is_pkg_init apimodel ∗
       "#Hisk" ∷ is_kubernetes γ l ∗
-      "%Hkind_eq" ∷ ⌜ kind = PureKObject.kind kobj ⌝ ∗
+      "%Hkind_eq" ∷ ⌜ kind = KObjectV.kind kobj ⌝ ∗
       "%Hnamespace_eq" ∷ ⌜ namespace = parent_key.(KKey.Namespace') ⌝ ∗
-      "%Hwf" ∷ ⌜ valid_create namespace kobj ⌝ ∗
+      "%Hwf" ∷ ⌜ KObjectV.valid_create namespace kobj ⌝ ∗
       "%Hparent_of" ∷ ⌜ obj_has_controller_parent_of kobj parent_key.(KKey.Kind') parent_key.(KKey.Name') parent_uid ⌝ ∗
-      "%Hkey_eq" ∷ ⌜ key = (PureKObject.key kobj) ⌝ ∗
-      "Hdeepown_i" ∷ PureKObject.deepown_i i kobj 1 ∗
+      "%Hkey_eq" ∷ ⌜ key = (KObjectV.key kobj) ⌝ ∗
+      "Hdeepown_i" ∷ KObjectV.deepown_i i kobj 1 ∗
       "Hfresh_key" ∷ own_fresh_key_frag γ key ∗
       "Hparent_meta" ∷ own_meta_frag γ parent_key parent_uid (Some parent_meta) ∗
       "Hchildren" ∷ own_weak_children_frag γ parent_key parent_uid children
   }}}
     l @ (ptrT.id apimodel.State.id) @ "create" #kind #namespace #i
   {{{ i' kobj' uid, RET (#i', #interface.nil);
-      ⌜ PureObjectMeta.created namespace (PureKObject.objectmeta kobj) (PureKObject.objectmeta kobj') ⌝ ∗
-      ⌜ PureObjectSpec.created (PureKObject.spec kobj) (PureKObject.spec kobj') ⌝ ∗
-      ⌜ PureObjectStatus.created (PureKObject.status kobj) (PureKObject.status kobj') ⌝ ∗
-      ⌜ valid kobj' ⌝ ∗
-      ⌜ key = (PureKObject.key kobj') ⌝ ∗
+      ⌜ ObjectMetaV.created namespace (KObjectV.objectmeta kobj) (KObjectV.objectmeta kobj') ⌝ ∗
+      ⌜ ObjectSpecV.created (KObjectV.spec kobj) (KObjectV.spec kobj') ⌝ ∗
+      ⌜ ObjectStatusV.created (KObjectV.status kobj) (KObjectV.status kobj') ⌝ ∗
+      ⌜ KObjectV.valid kobj' ⌝ ∗
+      ⌜ key = (KObjectV.key kobj') ⌝ ∗
       ⌜ key ∉ children ⌝ ∗
-      ⌜ uid = (PureKObject.objectmeta kobj').(PureObjectMeta.UID') ⌝ ∗
-      PureKObject.deepown_i i' kobj' 1 ∗
-      own_meta_frag γ key uid (Some (PureKObject.objectmeta kobj')) ∗
-      own_weak_spec_frag γ key uid (PureKObject.spec kobj') ∗
-      own_weak_status_frag γ key uid (PureKObject.status kobj') ∗
+      ⌜ uid = (KObjectV.objectmeta kobj').(ObjectMetaV.UID') ⌝ ∗
+      KObjectV.deepown_i i' kobj' 1 ∗
+      own_meta_frag γ key uid (Some (KObjectV.objectmeta kobj')) ∗
+      own_weak_spec_frag γ key uid (KObjectV.spec kobj') ∗
+      own_weak_status_frag γ key uid (KObjectV.status kobj') ∗
       own_meta_frag γ parent_key parent_uid (Some parent_meta) ∗
       own_weak_children_frag γ parent_key parent_uid (children ∪ {[key]}) ∗
       own_weak_children_frag γ key uid ∅ ∗
@@ -143,35 +137,33 @@ Proof. Admitted.
 Lemma wp_State__nameless_create γ l kind namespace i kobj parent_key parent_uid parent_meta children:
   {{{ is_pkg_init apimodel ∗
       "#Hisk" ∷ is_kubernetes γ l ∗
-      "%Hkind_eq" ∷ ⌜ kind = PureKObject.kind kobj ⌝ ∗
+      "%Hkind_eq" ∷ ⌜ kind = KObjectV.kind kobj ⌝ ∗
       "%Hnamespace_eq" ∷ ⌜ namespace = parent_key.(KKey.Namespace') ⌝ ∗
       "%Hparent_of" ∷ ⌜ obj_has_controller_parent_of kobj parent_key.(KKey.Kind') parent_key.(KKey.Name') parent_uid ⌝ ∗
-      "%Hwf" ∷ ⌜ valid_nameless_create namespace kobj ⌝ ∗
-      "Hdeepown_i" ∷ PureKObject.deepown_i i kobj 1 ∗
+      "%Hwf" ∷ ⌜ KObjectV.valid_nameless_create namespace kobj ⌝ ∗
+      "Hdeepown_i" ∷ KObjectV.deepown_i i kobj 1 ∗
       "Hparent_meta" ∷ own_meta_frag γ parent_key parent_uid (Some parent_meta) ∗
       "Hchildren" ∷ own_weak_children_frag γ parent_key parent_uid children
   }}}
     l @ (ptrT.id apimodel.State.id) @ "create" #kind #namespace #i
   {{{ i' kobj' key uid, RET (#i', #interface.nil);
-      ⌜ valid kobj' ⌝ ∗
-      ⌜ PureObjectMeta.nameless_created namespace (PureKObject.objectmeta kobj) (PureKObject.objectmeta kobj') ⌝ ∗
-      ⌜ PureObjectSpec.created (PureKObject.spec kobj) (PureKObject.spec kobj') ⌝ ∗
-      ⌜ PureObjectStatus.created (PureKObject.status kobj) (PureKObject.status kobj') ⌝ ∗
-      ⌜ key = (PureKObject.key kobj') ⌝ ∗
+      ⌜ KObjectV.valid kobj' ⌝ ∗
+      ⌜ ObjectMetaV.nameless_created namespace (KObjectV.objectmeta kobj) (KObjectV.objectmeta kobj') ⌝ ∗
+      ⌜ ObjectSpecV.created (KObjectV.spec kobj) (KObjectV.spec kobj') ⌝ ∗
+      ⌜ ObjectStatusV.created (KObjectV.status kobj) (KObjectV.status kobj') ⌝ ∗
+      ⌜ key = (KObjectV.key kobj') ⌝ ∗
       ⌜ key ∉ children ⌝ ∗
-      ⌜ uid = (PureKObject.objectmeta kobj').(PureObjectMeta.UID') ⌝ ∗
-      PureKObject.deepown_i i' kobj' 1 ∗
-      own_meta_frag γ key uid (Some (PureKObject.objectmeta kobj')) ∗
-      own_weak_spec_frag γ key uid (PureKObject.spec kobj') ∗
-      own_weak_status_frag γ key uid (PureKObject.status kobj') ∗
+      ⌜ uid = (KObjectV.objectmeta kobj').(ObjectMetaV.UID') ⌝ ∗
+      KObjectV.deepown_i i' kobj' 1 ∗
+      own_meta_frag γ key uid (Some (KObjectV.objectmeta kobj')) ∗
+      own_weak_spec_frag γ key uid (KObjectV.spec kobj') ∗
+      own_weak_status_frag γ key uid (KObjectV.status kobj') ∗
       own_meta_frag γ parent_key parent_uid (Some parent_meta) ∗
       own_weak_children_frag γ parent_key parent_uid (children ∪ {[key]}) ∗
       own_weak_children_frag γ key uid ∅ ∗
       own_snapshot_ro_frag_of γ kobj'
   }}}.
 Proof. Admitted.
-
-Axiom deleting: PureObjectMeta.t → PureObjectMeta.t → Prop.
 
 Lemma wp_State__delete γ l key uid kmeta parent_key parent_uid children:
   {{{ is_pkg_init apimodel ∗
@@ -181,8 +173,8 @@ Lemma wp_State__delete γ l key uid kmeta parent_key parent_uid children:
       "Hchildren" ∷ own_weak_children_frag γ parent_key parent_uid children
   }}}
     l @ (ptrT.id apimodel.State.id) @ "delete" #key #null #null
-  {{{ (kmeta': PureObjectMeta.t), RET #interface.nil;
-      (( ⌜ deleting kmeta kmeta' ⌝ ∗
+  {{{ (kmeta': ObjectMetaV.t), RET #interface.nil;
+      (( ⌜ ObjectMetaV.deleting kmeta kmeta' ⌝ ∗
           own_meta_frag γ key uid (Some kmeta') ∗
           own_weak_children_frag γ parent_key parent_uid children
         ) ∨
@@ -200,10 +192,10 @@ Lemma wp_State__delete_uid γ l key uid_ptr uid current_uid kmeta parent_key par
       "Hchildren" ∷ own_weak_children_frag γ parent_key parent_uid children
   }}}
     l @ (ptrT.id apimodel.State.id) @ "delete" #key #uid_ptr #null
-  {{{ (err: error.t) (kmeta': PureObjectMeta.t), RET #err;
+  {{{ (err: error.t) (kmeta': ObjectMetaV.t), RET #err;
       ( ⌜ uid = current_uid ⌝ ∗
         ⌜ err = interface.nil ⌝ ∗
-        ((⌜ deleting kmeta kmeta' ⌝ ∗
+        ((⌜ ObjectMetaV.deleting kmeta kmeta' ⌝ ∗
             own_meta_frag γ key current_uid (Some kmeta') ∗
             own_weak_children_frag γ parent_key parent_uid children
           ) ∨
@@ -227,55 +219,49 @@ Lemma wp_State__delete_rv γ l key uid_ptr uid rv_ptr rv prev_kobj current_uid k
       "Hchildren" ∷ own_weak_children_frag γ parent_key parent_uid children
   }}}
     l @ (ptrT.id apimodel.State.id) @ "delete" #key #uid_ptr #rv_ptr
-  {{{ (err: error.t) (kmeta': PureObjectMeta.t), RET #err;
+  {{{ (err: error.t) (kmeta': ObjectMetaV.t), RET #err;
       ( ⌜ uid = current_uid ⌝ ∗
-        ⌜ rv = kmeta.(PureObjectMeta.ResourceVersion') ⌝ ∗
+        ⌜ rv = kmeta.(ObjectMetaV.ResourceVersion') ⌝ ∗
         ⌜ err = interface.nil ⌝ ∗
-        ((⌜ deleting kmeta kmeta' ⌝ ∗
+        ((⌜ ObjectMetaV.deleting kmeta kmeta' ⌝ ∗
             own_meta_frag γ key current_uid (Some kmeta') ∗
             own_weak_children_frag γ parent_key parent_uid children
           ) ∨
           own_weak_children_frag γ parent_key parent_uid (children ∖ {[key]})
         )
       ) ∨
-      ( (⌜ uid ≠ current_uid ⌝ ∨ ⌜ rv ≠ kmeta.(PureObjectMeta.ResourceVersion') ⌝) ∗
+      ( (⌜ uid ≠ current_uid ⌝ ∨ ⌜ rv ≠ kmeta.(ObjectMetaV.ResourceVersion') ⌝) ∗
         ⌜ err ≠ interface.nil ⌝
       )
   }}}.
 Proof. Admitted.
 
-(* update satisfies Kubernetes update invariant *)
-Axiom valid_update: go_string → PureKObject.t → PureKObject.t → Prop.
-
-(* update from the old meta to the new meta doesn't modify owner references and doesn't trigger deletion *)
-Axiom simple_update: PureObjectMeta.t → PureObjectMeta.t → Prop.
-
 Lemma wp_State__update γ l kind namespace i key uid rv prev_kobj kobj kmeta kspec:
   {{{ is_pkg_init apimodel ∗
       "#Hisk" ∷ is_kubernetes γ l ∗
       "#Hsnapshot" ∷ own_snapshot_ro_frag γ key uid rv prev_kobj ∗
-      "%Hkind_eq" ∷ ⌜ kind = PureKObject.kind kobj ⌝ ∗
-      "%Hkey_eq" ∷ ⌜ key = PureKObject.key kobj ⌝ ∗
-      "%Hv" ∷ ⌜ valid kobj ⌝ ∗
-      "%Hvu" ∷ ⌜ valid_update namespace prev_kobj kobj ⌝ ∗
-      "%Hsu" ∷ ⌜ simple_update (PureKObject.objectmeta prev_kobj) (PureKObject.objectmeta kobj) ⌝ ∗
-      "Hdeepown_i" ∷ PureKObject.deepown_i i kobj 1 ∗
+      "%Hkind_eq" ∷ ⌜ kind = KObjectV.kind kobj ⌝ ∗
+      "%Hkey_eq" ∷ ⌜ key = KObjectV.key kobj ⌝ ∗
+      "%Hv" ∷ ⌜ KObjectV.valid kobj ⌝ ∗
+      "%Hvu" ∷ ⌜ KObjectV.valid_update namespace prev_kobj kobj ⌝ ∗
+      "%Hsu" ∷ ⌜ ObjectMetaV.simple_update (KObjectV.objectmeta prev_kobj) (KObjectV.objectmeta kobj) ⌝ ∗
+      "Hdeepown_i" ∷ KObjectV.deepown_i i kobj 1 ∗
       "Hmeta" ∷ own_meta_frag γ key uid (Some kmeta) ∗
       "Hspec" ∷ own_weak_spec_frag γ key uid kspec
   }}}
     l @ (ptrT.id apimodel.State.id) @ "update" #kind #namespace #i
   {{{ i' (err: error.t) kobj', RET (#i', #err);
-      ( ⌜ kmeta.(PureObjectMeta.ResourceVersion') = rv ⌝ ∗
+      ( ⌜ kmeta.(ObjectMetaV.ResourceVersion') = rv ⌝ ∗
         ⌜ err = interface.nil ⌝ ∗
-        ⌜ valid kobj' ⌝ ∗
-        ⌜ PureObjectMeta.updated kmeta (PureKObject.objectmeta kobj) (PureKObject.objectmeta kobj') ⌝ ∗
-        ⌜ PureObjectSpec.updated kspec (PureKObject.spec kobj) (PureKObject.spec kobj') ⌝ ∗
-        PureKObject.deepown_i i' kobj' 1 ∗
-        own_meta_frag γ key uid (Some (PureKObject.objectmeta kobj')) ∗
-        own_weak_spec_frag γ key uid (PureKObject.spec kobj') ∗
+        ⌜ KObjectV.valid kobj' ⌝ ∗
+        ⌜ ObjectMetaV.updated kmeta (KObjectV.objectmeta kobj) (KObjectV.objectmeta kobj') ⌝ ∗
+        ⌜ ObjectSpecV.updated kspec (KObjectV.spec kobj) (KObjectV.spec kobj') ⌝ ∗
+        KObjectV.deepown_i i' kobj' 1 ∗
+        own_meta_frag γ key uid (Some (KObjectV.objectmeta kobj')) ∗
+        own_weak_spec_frag γ key uid (KObjectV.spec kobj') ∗
         own_snapshot_ro_frag_of γ kobj'
       ) ∨ (
-        ⌜ kmeta.(PureObjectMeta.ResourceVersion') ≠ rv ⌝ ∗
+        ⌜ kmeta.(ObjectMetaV.ResourceVersion') ≠ rv ⌝ ∗
         ⌜ err ≠ interface.nil ⌝ ∗
         own_meta_frag γ key uid (Some kmeta) ∗
         own_weak_spec_frag γ key uid kspec
